Translate and prove atomic.Int32; add and use primitive spec for AtomicOp

new/proof/sync/atomic.v
@@ -40,7 +40,13 @@ Lemma wp_AddUint64 (addr : loc) (v : w64) :
   (|={⊤,∅}=> ∃ (oldv : w64), addr ↦ oldv ∗ (addr ↦ (word.add oldv v) ={∅,⊤}=∗ Φ #(word.add oldv v))) -∗
   WP atomic @ "AddUint64" #addr #v {{ Φ }}.
 Proof.
-Admitted.
+  wp_start as "_".
+  iMod "HΦ" as (?) "[Haddr HΦ]".
+  rewrite typed_pointsto_unseal /typed_pointsto_def /=.
+  rewrite to_val_unseal /=. rewrite loc_add_0 !right_id.
+  iApply (wp_atomic_op with "Haddr"); first done.
+  iFrame.
+Qed.
 
 Lemma wp_CompareAndSwapUint64 (addr : loc) (old : w64) (new : w64) :
   ∀ Φ,
@@ -52,6 +58,72 @@ Lemma wp_CompareAndSwapUint64 (addr : loc) (old : w64) (new : w64) :
      (addr ↦{dq} (if decide (v = old) then new else v) ={∅,⊤}=∗ Φ #(bool_decide (v = old)))
   ) -∗
   WP atomic @ "CompareAndSwapUint64" #addr #old #new {{ Φ }}.
+Proof.
+  wp_start as "_".
+  wp_bind (CmpXchg _ _ _).
+  iMod "HΦ" as (??) "(? & -> & HΦ)".
+  rewrite bool_decide_decide.
+  destruct decide.
+  {
+    subst.
+    unshelve iApply (wp_typed_cmpxchg_suc with "[$]"); try tc_solve; try done.
+    iIntros "!> ?". iMod ("HΦ" with "[$]"). iModIntro.
+    by wp_auto.
+  }
+  {
+    unshelve iApply (wp_typed_cmpxchg_fail with "[$]"); try tc_solve; try done.
+    { naive_solver. }
+    iIntros "!> ?". iMod ("HΦ" with "[$]"). iModIntro.
+    by wp_auto.
+  }
+Qed.
+
+Lemma wp_LoadInt32 (addr : loc) dq :
+  ∀ Φ,
+  is_pkg_init atomic -∗
+  (|={⊤,∅}=> ∃ (v : w32), addr ↦{dq} v ∗ (addr ↦{dq} v ={∅,⊤}=∗ Φ #v)) -∗
+  WP atomic @ "LoadInt32" #addr {{ Φ }}.
+Proof.
+  wp_start as "_".
+  iMod "HΦ" as (?) "[Haddr HΦ]".
+  unshelve iApply (wp_typed_Load with "[$]"); try tc_solve; done.
+Qed.
+
+Lemma wp_StoreInt32 (addr : loc) (v : w32) :
+  ∀ Φ,
+  is_pkg_init atomic -∗
+  (|={⊤,∅}=> ∃ (oldv : w32), addr ↦ oldv ∗ (addr ↦ v ={∅,⊤}=∗ Φ #())) -∗
+  WP atomic @ "StoreInt32" #addr #v {{ Φ }}.
+Proof.
+  wp_start as "_".
+  iMod "HΦ" as (?) "[Haddr HΦ]".
+  unshelve iApply (wp_typed_AtomicStore with "[$]"); try tc_solve; done.
+Qed.
+
+Lemma wp_AddInt32 (addr : loc) (v : w32) :
+  ∀ Φ,
+  is_pkg_init atomic -∗
+  (|={⊤,∅}=> ∃ (oldv : w32), addr ↦ oldv ∗ (addr ↦ (word.add oldv v) ={∅,⊤}=∗ Φ #(word.add oldv v))) -∗
+  WP atomic @ "AddInt32" #addr #v {{ Φ }}.
+Proof.
+  wp_start as "_".
+  iMod "HΦ" as (?) "[Haddr HΦ]".
+  rewrite typed_pointsto_unseal /typed_pointsto_def /=.
+  rewrite to_val_unseal /=. rewrite loc_add_0 !right_id.
+  iApply (wp_atomic_op with "Haddr"); first done.
+  iFrame.
+Qed.
+
+Lemma wp_CompareAndSwapInt32 (addr : loc) (old : w32) (new : w32) :
+  ∀ Φ,
+  is_pkg_init atomic -∗
+  (|={⊤,∅}=>
+     ∃ (v: w32) dq,
+     addr ↦{dq} v ∗
+     ⌜ dq = if decide (v = old) then DfracOwn 1 else dq ⌝ ∗
+     (addr ↦{dq} (if decide (v = old) then new else v) ={∅,⊤}=∗ Φ #(bool_decide (v = old)))
+  ) -∗
+  WP atomic @ "CompareAndSwapInt32" #addr #old #new {{ Φ }}.
 Proof.
   wp_start as "_".
   wp_bind (CmpXchg _ _ _).
@@ -101,6 +173,7 @@ Proof.
   iModIntro.
   wp_auto. done.
 Qed.
+
 
 Lemma wp_Uint64__Store u v :
   ∀ Φ,
@@ -183,6 +256,124 @@ Proof.
   {
     (* FIXME: StructFieldsSplit typeclass is shelved unless something is specified up front. *)
     iApply (struct_fields_combine (V:=atomic.Uint64.t)).
+    iFrame.
+  }
+  iModIntro.
+  wp_auto. done.
+Qed.
+
+Definition own_Int32 (u : loc) dq (v : w32) : iProp Σ :=
+  u ↦{dq} atomic.Int32.mk (default_val _) v.
+
+Lemma wp_Int32__Load u dq :
+  ∀ Φ,
+  is_pkg_init atomic -∗
+  (|={⊤,∅}=> ∃ v, own_Int32 u dq v ∗ (own_Int32 u dq v ={∅,⊤}=∗ Φ #v)) -∗
+  WP u @ atomic @ "Int32'ptr" @ "Load" #() {{ Φ }}.
+Proof.
+  wp_start as "_".
+  wp_auto.
+  wp_apply (wp_LoadInt32 with "[$]").
+  iMod "HΦ". iModIntro.
+  iDestruct "HΦ" as (?) "[Hown HΦ]".
+
+  iDestruct (struct_fields_split with "Hown") as "Hl".
+  iNamed "Hl". simpl.
+  iExists _. iFrame.
+  iIntros "Hv".
+
+  iMod ("HΦ" with "[-]").
+  {
+    (* FIXME: StructFieldsSplit typeclass is shelved unless something is specified up front. *)
+    iApply (struct_fields_combine (V:=atomic.Int32.t)).
+    iFrame.
+  }
+  iModIntro.
+  wp_auto. done.
+Qed.
+
+
+Lemma wp_Int32__Store u v :
+  ∀ Φ,
+  is_pkg_init atomic -∗
+  (|={⊤,∅}=> ∃ old, own_Int32 u (DfracOwn 1) old ∗ (own_Int32 u (DfracOwn 1) v ={∅,⊤}=∗ Φ #())) -∗
+  WP u @ atomic @ "Int32'ptr" @ "Store" #v {{ Φ }}.
+Proof.
+  wp_start as "_".
+  wp_auto.
+  wp_apply (wp_StoreInt32 with "[$]").
+  iMod "HΦ". iModIntro.
+  iDestruct "HΦ" as (?) "[Hown HΦ]".
+
+  iDestruct (struct_fields_split with "Hown") as "Hl".
+  iNamed "Hl". simpl.
+  iExists _. iFrame.
+  iIntros "Hv".
+
+  iMod ("HΦ" with "[-]").
+  {
+    (* FIXME: StructFieldsSplit typeclass is shelved unless something is specified up front. *)
+    iApply (struct_fields_combine (V:=atomic.Int32.t)).
+    iFrame.
+  }
+  iModIntro.
+  wp_auto. done.
+Qed.
+
+Lemma wp_Int32__Add u delta :
+  ∀ Φ,
+  is_pkg_init atomic -∗
+  (|={⊤,∅}=> ∃ old, own_Int32 u (DfracOwn 1) old ∗
+  (own_Int32 u (DfracOwn 1) (word.add old delta) ={∅,⊤}=∗
+   Φ #(word.add old delta))) -∗
+  WP u @ atomic @ "Int32'ptr" @ "Add" #delta {{ Φ }}.
+Proof.
+  wp_start as "_".
+  wp_auto.
+  wp_apply (wp_AddInt32 with "[$]").
+  iMod "HΦ". iModIntro.
+  iDestruct "HΦ" as (?) "[Hown HΦ]".
+
+  iDestruct (struct_fields_split with "Hown") as "Hl".
+  iNamed "Hl". simpl.
+  iExists _. iFrame.
+  iIntros "Hv".
+
+  iMod ("HΦ" with "[-]").
+  {
+    (* FIXME: StructFieldsSplit typeclass is shelved unless something is specified up front. *)
+    iApply (struct_fields_combine (V:=atomic.Int32.t)).
+    iFrame.
+  }
+  iModIntro.
+  wp_auto. done.
+Qed.
+
+Lemma wp_Int32__CompareAndSwap u old new :
+  ∀ Φ,
+  is_pkg_init atomic -∗
+  (|={⊤,∅}=> ∃ v dq, own_Int32 u dq v ∗
+                    ⌜ dq = if decide (v = old) then DfracOwn 1 else dq ⌝ ∗
+  (own_Int32 u dq (if decide (v = old) then new else v) ={∅,⊤}=∗ Φ #(bool_decide (v = old)))) -∗
+  WP u @ atomic @ "Int32'ptr" @ "CompareAndSwap" #old #new {{ Φ }}.
+Proof.
+  wp_start as "_".
+  wp_auto.
+  wp_apply (wp_CompareAndSwapInt32 with "[$]").
+  iMod "HΦ". iModIntro.
+  iDestruct "HΦ" as (??) "(Hown & -> & HΦ)".
+
+  iDestruct (struct_fields_split with "Hown") as "Hl".
+  iNamed "Hl". simpl.
+  iExists _. iFrame.
+  iSplitR.
+  { by destruct decide. }
+  iIntros "Hv".
+
+  iMod ("HΦ" with "[-]").
+  {
+    (* FIXME: StructFieldsSplit typeclass is shelved unless something is specified up front. *)
+    iApply (struct_fields_combine (V:=atomic.Int32.t)).
     iFrame.
   }
   iModIntro.
