new/trusted_code/sync/atomic.v
@@ -11,12 +11,24 @@ Definition StoreUint64 : val :=
   λ: "addr" "val", AtomicStore "addr" "val".
 
 Definition AddUint64 : val :=
-  λ: "addr", #() #().
+  λ: "addr" "val", AtomicOp PlusOp "addr" "val".
 
 Definition CompareAndSwapUint64 : val :=
   λ: "addr" "old" "new",
-    Snd (CmpXchg "addr" "old" "new")
-.
+    Snd (CmpXchg "addr" "old" "new").
+
+Definition LoadInt32 : val :=
+  λ: "addr", Load "addr".
+
+Definition StoreInt32 : val :=
+  λ: "addr" "val", AtomicStore "addr" "val".
+
+Definition AddInt32 : val :=
+  λ: "addr" "val", AtomicOp PlusOp "addr" "val".
+
+Definition CompareAndSwapInt32 : val :=
+  λ: "addr" "old" "new",
+    Snd (CmpXchg "addr" "old" "new").
 
 End code.
 End atomic.
